src/Examples/Numeric/Example_Interval_Loop_Coverage.thy
@@ -42,27 +42,36 @@ subsection \<open>The compiled CFG\<close>
 abbreviation "loop_cfg \<equiv> compile_prog Map.empty [] ''main'' loop_prog"
 
 lemma loop_cfg_full:
-  "loop_cfg = mk_cfg 0 5
-     {(0, EA_Assign ''x'' (N 0), 1),
-      (1, EA_Nop, 2),
-      (2, EA_Assume (Less (V ''x'') (N 20)), 3),
-      (2, EA_AssumeNot (Less (V ''x'') (N 20)), 5),
-      (3, EA_Assign ''x'' (Plus (V ''x'') (N 1)), 4),
-      (4, EA_Nop, 2)}
-     {}"
-  by (simp add: compile_prog_def compile_prog_with_regions_def compile_procs_list_def Let_def eval_nat_numeral loop_prog_def; blast)
+  "loop_cfg =
+     \<lparr> intra =
+         {(FunctionEntry ''main'', EA_Nop, Statement 0),
+          (Statement 0, EA_Assign ''x'' (N 0), Statement 1),
+          (Statement 1, EA_Nop, Statement 2),
+          (Statement 2, EA_Assume (Less (V ''x'') (N 20)), Statement 3),
+          (Statement 2, EA_AssumeNot (Less (V ''x'') (N 20)), Statement 5),
+          (Statement 3, EA_Assign ''x'' (Plus (V ''x'') (N 1)), Statement 4),
+          (Statement 4, EA_Nop, Statement 2),
+          (Statement 5, EA_Ret None ''main'', FunctionResult ''main'')},
+       calls = {},
+       cfg_entry = FunctionEntry ''main'' \<rparr>"
+  by eval
 
-lemma loop_cfg_entry:   "cfg_entry loop_cfg = 0" by (simp add: loop_cfg_full)
-lemma loop_cfg_exit:    "cfg_exit  loop_cfg = 5" by (simp add: loop_cfg_full)
-lemma loop_cfg_combines: "combines loop_cfg = {}" by (simp add: loop_cfg_full)
-lemma loop_cfg_edges:
-  "edges loop_cfg =
-     {(0, EA_Assign ''x'' (N 0), 1),
-      (1, EA_Nop, 2),
-      (2, EA_Assume (Less (V ''x'') (N 20)), 3),
-      (2, EA_AssumeNot (Less (V ''x'') (N 20)), 5),
-      (3, EA_Assign ''x'' (Plus (V ''x'') (N 1)), 4),
-      (4, EA_Nop, 2)}"
+lemma loop_cfg_entry: "cfg_entry loop_cfg = FunctionEntry ''main''"
+  by (simp add: loop_cfg_full)
+lemma loop_cfg_exit: "cfg_exit loop_cfg = FunctionResult ''main''"
+  by (simp add: loop_cfg_full cfg_exit_def)
+lemma loop_cfg_calls: "calls loop_cfg = {}"
+  by (simp add: loop_cfg_full)
+lemma loop_cfg_intra:
+  "intra loop_cfg =
+     {(FunctionEntry ''main'', EA_Nop, Statement 0),
+      (Statement 0, EA_Assign ''x'' (N 0), Statement 1),
+      (Statement 1, EA_Nop, Statement 2),
+      (Statement 2, EA_Assume (Less (V ''x'') (N 20)), Statement 3),
+      (Statement 2, EA_AssumeNot (Less (V ''x'') (N 20)), Statement 5),
+      (Statement 3, EA_Assign ''x'' (Plus (V ''x'') (N 1)), Statement 4),
+      (Statement 4, EA_Nop, Statement 2),
+      (Statement 5, EA_Ret None ''main'', FunctionResult ''main'')}"
   by (simp add: loop_cfg_full)
 
 subsection \<open>An exhibited interval post-fixpoint\<close>
@@ -79,31 +88,51 @@ text \<open>
 \<close>
 definition loop_env :: "pp \<Rightarrow> ivl abs_state" where
   "loop_env v =
-     (if v = 1 then (\<lambda>_. Ivl MinInf PlusInf)(''x'' := Ivl (Fin 0) (Fin 0))
-      else if v = 3 then (\<lambda>_. Ivl MinInf PlusInf)(''x'' := Ivl (Fin 0) (Fin 19))
-      else if v = 4 then (\<lambda>_. Ivl MinInf PlusInf)(''x'' := Ivl (Fin 1) (Fin 20))
-      else if v \<in> {2,5} then (\<lambda>_. Ivl MinInf PlusInf)(''x'' := Ivl (Fin 0) (Fin 20))
+     (if v = Statement 1 then (\<lambda>_. Ivl MinInf PlusInf)(''x'' := Ivl (Fin 0) (Fin 0))
+      else if v = Statement 3 then (\<lambda>_. Ivl MinInf PlusInf)(''x'' := Ivl (Fin 0) (Fin 19))
+      else if v = Statement 4 then (\<lambda>_. Ivl MinInf PlusInf)(''x'' := Ivl (Fin 1) (Fin 20))
+      else if v \<in> {Statement 2, Statement 5}
+        then (\<lambda>_. Ivl MinInf PlusInf)(''x'' := Ivl (Fin 0) (Fin 20))
       else (\<lambda>_. Ivl MinInf PlusInf))"
+
+text \<open>The program is call-free, so both call-shaped sources of \<^const>\<open>rhs\<close> are empty and
+  only the intra predecessors constrain \<^const>\<open>loop_env\<close>.\<close>
+
+lemma loop_entry_calls: "entry_calls loop_cfg v = {}"
+  by (simp add: entry_calls_def loop_cfg_calls)
+
+lemma loop_return_calls: "return_calls loop_cfg v = {}"
+  by (simp add: return_calls_def loop_cfg_calls)
+
+lemma loop_intra_predecessors_finite: "finite (intra_predecessors loop_cfg v)"
+  by (rule finite_intra_predecessors) (simp add: loop_cfg_intra)
 
 lemma loop_postfix:
   "is_post_fixpoint loop_cfg ivl_tf (\<squnion>) bot loop_s0 loop_env"
   unfolding is_post_fixpoint_def
 proof (rule allI)
   fix v
-  show "rhs loop_cfg ivl_tf (\<squnion>) bot loop_s0 loop_env v \<le> loop_env v"
-    apply (simp only: rhs_def Let_def loop_cfg_entry loop_cfg_edges loop_cfg_combines)
-    apply (rule abs_join_set_le)
-    apply (rule finite_subset[where B=
-            "insert loop_s0 ((\<lambda>(u,a). apply_tf ivl_tf a (loop_env u)) `
-               {(0, EA_Assign ''x'' (N 0)),
-                (1, EA_Nop),
-                (2, EA_Assume (Less (V ''x'') (N 20))),
-                (2, EA_AssumeNot (Less (V ''x'') (N 20))),
-                (3, EA_Assign ''x'' (Plus (V ''x'') (N 1))),
-                (4, EA_Nop)})"])
+  let ?I = "(\<lambda>(u, a). apply_tf ivl_tf a (loop_env u)) ` intra_predecessors loop_cfg v"
+  have finI: "finite ?I" using loop_intra_predecessors_finite by blast
+  have leI: "\<And>t. t \<in> ?I \<Longrightarrow> t \<le> loop_env v"
     by (auto split: if_splits
-             simp: loop_env_def loop_s0_def ivl_tf_def assign_ivl_def
-                   assume_ivl_def assume_not_ivl_def normalize_ivl_def less_eq_ivl_def le_fun_def)
+             simp: intra_predecessors_def loop_cfg_intra loop_env_def ivl_tf_def
+                   assign_ivl_def assume_ivl_def assume_not_ivl_def normalize_ivl_def
+                   less_eq_ivl_def le_fun_def)
+  show "rhs loop_cfg ivl_tf (\<squnion>) bot loop_s0 loop_env v \<le> loop_env v"
+  proof (cases "v = cfg_entry loop_cfg")
+    case True
+    then have "loop_s0 \<le> loop_env v"
+      by (simp add: loop_cfg_entry loop_s0_def loop_env_def)
+    with True finI leI show ?thesis
+      unfolding rhs_def Let_def loop_entry_calls loop_return_calls
+      by (auto intro!: abs_join_set_le)
+  next
+    case False
+    with finI leI show ?thesis
+      unfolding rhs_def Let_def loop_entry_calls loop_return_calls
+      by (auto intro!: abs_join_set_le)
+  qed
 qed
 
 subsection \<open>Backward guard refinement at the body entry\<close>
@@ -116,10 +145,10 @@ text \<open>
   @{text "Example_Guard_Refinement"}).
 \<close>
 
-abbreviation "loop_body_entry \<equiv> 3"
+abbreviation "loop_body_entry \<equiv> Statement 3"
 
 lemma loop_body_x_from_assume:
-  "tf_assume ivl_tf (Less (V ''x'') (N 20)) (loop_env 2) ''x'' = Ivl (Fin 0) (Fin 19)"
+  "tf_assume ivl_tf (Less (V ''x'') (N 20)) (loop_env (Statement 2)) ''x'' = Ivl (Fin 0) (Fin 19)"
   unfolding ivl_tf_def assume_ivl_def loop_env_def
   by (simp add: inv_less_ivl.simps ivl_backward_domain.bfilter.simps
         ivl_backward_domain.afilter.simps aval_ivl.simps aval_ivl_hol.simps meet_ivl.simps)
@@ -131,15 +160,15 @@ lemma loop_body_entry_x:
 subsection \<open>Soundness: @{text "0 \<le> x \<le> 20"} at the loop head\<close>
 
 text \<open>The loop head is the assume node where @{term \<open>x < 20\<close>} is checked.\<close>
-abbreviation "loop_head \<equiv> 2"
+abbreviation "loop_head \<equiv> Statement 2"
 
 lemma loop_head_x_bounded:
   assumes S_sound: "S \<subseteq> \<lbrakk>loop_s0\<rbrakk>"
   assumes s: "s \<in> ltr_collect loop_cfg S loop_head"
   shows "0 \<le> s ''x'' \<and> s ''x'' \<le> 20"
 proof -
-  have fin_e: "finite (edges loop_cfg)" by (simp add: loop_cfg_edges)
-  have fin_c: "finite (combines loop_cfg)" by (simp add: loop_cfg_combines)
+  have fin_e: "finite (intra loop_cfg)" by (simp add: loop_cfg_intra)
+  have fin_c: "finite (calls loop_cfg)" by (simp add: loop_cfg_calls)
   have le: "ltr_collect loop_cfg S loop_head \<le> \<lbrakk>loop_env loop_head\<rbrakk>"
     using sound_transfer.unified_ltr_post_fixpoint_sound
           [OF ivl_sound_tf.sound_transfer_axioms fin_e fin_c loop_postfix S_sound]
